src/ldrfpf/LocalPF.v
@@ -25,7 +25,9 @@ Require Import Pred.
 Require Import Trace.
 
 Require Import PromiseConsistent.
+Require Import PFConsistent.
 Require Import MemoryProps.
+Require Import Single.
 
 Set Implicit Arguments.
 
@@ -44,6 +46,531 @@ Section LOCALPF.
       (<<CONSISTENT: Trace.consistent th tr_cert>>) /\
       (<<PFCERT: List.Forall (compose pf_event snd) tr_cert>>).
 
+  Lemma pf_consistent_consistent lang (th: Thread.t lang)
+        (CONSISTENT: pf_consistent th)
+    :
+      Thread.consistent th.
+  Proof.
+    ii. unfold pf_consistent in *. des.
+    exploit CONSISTENT0; eauto. i. des.
+    { eapply Trace.silent_steps_tau_steps in STEPS; eauto.
+      left. unfold Thread.steps_failure. esplits; eauto. }
+    { eapply Trace.silent_steps_tau_steps in STEPS; eauto. }
+  Qed.
+
+
+  (* a single thread steps per one configuration step *)
+  Inductive pf_step:
+    forall (e:ThreadEvent.t) (tid:Ident.t) (c1 c2:Configuration.t), Prop :=
+  | pf_step_intro
+      e tid c1 lang st1 lc1 e2 e3 st4 lc4 sc4 memory4
+      (TID: IdentMap.find tid c1.(Configuration.threads) = Some (existT _ lang st1, lc1))
+      (CANCELS: rtc (@Thread.cancel_step _) (Thread.mk _ st1 lc1 c1.(Configuration.sc) c1.(Configuration.memory)) e2)
+      (STEP: Thread.opt_step e e2 e3)
+      (RESERVES: rtc (@Thread.reserve_step _) e3 (Thread.mk _ st4 lc4 sc4 memory4))
+      (CONSISTENT: e <> ThreadEvent.failure -> pf_consistent (Thread.mk _ st4 lc4 sc4 memory4))
+      (PF: pf_event e)
+    :
+      pf_step e tid c1 (Configuration.mk (IdentMap.add tid (existT _ _ st4, lc4) c1.(Configuration.threads)) sc4 memory4)
+  .
+  Hint Constructors pf_step.
+
+  Inductive pf_machine_step: forall (e:MachineEvent.t) (tid:Ident.t) (c1 c2:Configuration.t), Prop :=
+  | pf_machine_step_intro
+      e tid c1 c2
+      (STEP: pf_step e tid c1 c2)
+    :
+      pf_machine_step (ThreadEvent.get_machine_event e) tid c1 c2
+  .
+  Hint Constructors pf_machine_step.
+
+  Inductive opt_pf_machine_step:
+    forall (e: MachineEvent.t) (tid: Ident.t) (c1 c2: Configuration.t), Prop :=
+  | opt_pf_machine_step_none
+      tid c:
+      opt_pf_machine_step MachineEvent.silent tid c c
+  | opt_pf_machine_step_some
+      e tid c1 c2
+      (STEP: pf_machine_step e tid c1 c2):
+      opt_pf_machine_step e tid c1 c2
+  .
+  Hint Constructors opt_pf_machine_step.
+
+  Definition tau_pf_machine_step := union (pf_machine_step MachineEvent.silent).
+
+  Inductive pf_all_step (c1 c2: Configuration.t): Prop :=
+  | pf_all_step_intro
+      e tid
+      (STEP: pf_step e tid c1 c2)
+  .
+  Hint Constructors pf_all_step.
+
+  Inductive pf_steps:
+    forall (es: list ThreadEvent.t) (tid: Ident.t) (c1 c2:Configuration.t), Prop :=
+  | pf_steps_nil
+      tid c1
+    :
+      pf_steps [] tid c1 c1
+  | pf_steps_cons
+      ehd etl tid c1 c2 c3
+      (STEP: pf_step ehd tid c1 c2)
+      (STEPS: pf_steps etl tid c2 c3)
+    :
+      pf_steps (ehd :: etl) tid c1 c3
+  .
+  Hint Constructors pf_steps.
+
+  Lemma pf_steps_rtc_pf_all_step es tid c1 c2
+        (STEPS: pf_steps es tid c1 c2)
+    :
+      rtc pf_all_step c1 c2.
+  Proof.
+    induction STEPS; eauto.
+  Qed.
+
+  Lemma pf_steps_split es0 es1 tid c0 c2
+        (STEPS: pf_steps (es0 ++ es1) tid c0 c2)
+    :
+      exists c1,
+        (<<STEPS0: pf_steps es0 tid c0 c1>>) /\
+        (<<STEPS1: pf_steps es1 tid c1 c2>>).
+  Proof.
+    ginduction es0; eauto. i. ss. inv STEPS.
+    exploit IHes0; eauto. i. des.
+    esplits; eauto.
+  Qed.
+
+  Lemma silent_pf_steps_tau_pf_machine_steps es tid c1 c2
+        (STEPS: pf_steps es tid c1 c2)
+        (SILENT: List.Forall (fun e => ThreadEvent.get_machine_event e = MachineEvent.silent) es)
+    :
+      rtc (pf_machine_step MachineEvent.silent tid) c1 c2.
+  Proof.
+    ginduction es; i.
+    { inv STEPS. eauto. }
+    { inv STEPS. inv SILENT. exploit IHes; eauto.
+      i. econs 2; eauto. rewrite <- H1. econs; eauto. }
+  Qed.
+
+  Inductive reading_event (loc: Loc.t) (ts: Time.t):
+    forall (e: ThreadEvent.t), Prop :=
+  | reading_event_read
+      valr releasedr ordr
+    :
+      reading_event loc ts (ThreadEvent.read loc ts valr releasedr ordr)
+  | reading_event_update
+      to valr valw releasedr releasedw ordr ordw
+    :
+      reading_event loc ts (ThreadEvent.update loc ts to valr valw releasedr releasedw ordr ordw)
+  .
+
+  Inductive writing_event (loc: Loc.t) (ts: Time.t):
+    forall (e: ThreadEvent.t), Prop :=
+  | writing_event_write
+      from valw releasedw ordw
+      (ORD: Ordering.le ordw Ordering.relaxed)
+    :
+      writing_event loc ts (ThreadEvent.write loc from ts valw releasedw ordw)
+  | writing_event_update
+      from valr valw releasedr releasedw ordr ordw
+      (ORD: Ordering.le ordw Ordering.relaxed)
+    :
+      writing_event loc ts (ThreadEvent.update loc from ts valr valw releasedr releasedw ordr ordw)
+  .
+
+  Definition pf_racefree_imm (c0: Configuration.t): Prop :=
+    forall tid0 c1 tid1 c2 c3
+           loc ts te0 te1 e0 e1
+           (LOC: L loc)
+           (TID: tid0 <> tid1)
+           (CSTEP0: pf_step e0 tid0 c0 c1)
+           (WRITE: writing_event loc ts te0)
+           (STEPS: rtc (pf_machine_step MachineEvent.silent tid1) c1 c2)
+           (CSTEP1: pf_step e1 tid1 c2 c3)
+           (READ: reading_event loc ts te1),
+      False.
+
+  Definition pf_racefree (c0: Configuration.t): Prop :=
+    forall c1
+           (CSTEPS: rtc pf_all_step c0 c1),
+      pf_racefree_imm c1.
+
+  Lemma step_pf_racefree c0 c1 e tid
+        (RACEFREE: pf_racefree c0)
+        (STEP: pf_step e tid c0 c1)
+    :
+      pf_racefree c1.
+  Proof.
+    unfold pf_racefree in *. i.
+    eapply RACEFREE. econs 2; eauto.
+  Qed.
+
+  Lemma rtc_tau_machine_step_pf_racefree c0 c1
+        (RACEFREE: pf_racefree c0)
+        (STEP: rtc tau_pf_machine_step c0 c1)
+    :
+      pf_racefree c1.
+  Proof.
+    ginduction STEP; eauto.
+    i. eapply IHSTEP. inv H. inv USTEP.
+    eapply step_pf_racefree; eauto.
+  Qed.
+
+  Lemma steps_pf_racefree es tid c0 c1
+        (RACEFREE: pf_racefree c0)
+        (STEPS: pf_steps es tid c0 c1)
+    :
+      pf_racefree c1.
+  Proof.
+    ginduction STEPS; eauto.
+    i. eapply IHSTEPS.
+    eapply step_pf_racefree; eauto.
+  Qed.
+
+  Definition pf_promises (prom: Memory.t): Prop :=
+    forall loc to from msg
+           (LOC: L loc)
+           (GET: Memory.get loc to prom = Some (from, msg)),
+      msg = Message.reserve.
+
+  Lemma pf_promises_promise prom0 mem0 loc from to msg prom1 mem1 kind
+        (PROMISE: Memory.promise prom0 mem0 loc from to msg prom1 mem1 kind)
+        (PF: L loc -> msg = Message.reserve)
+        (PROMISES: pf_promises prom0)
+    :
+      pf_promises prom1.
+  Proof.
+    inv PROMISE.
+    - ii. erewrite Memory.add_o in GET; eauto. des_ifs.
+      + ss. des; clarify. auto.
+      + eapply PROMISES; eauto.
+    - ii. erewrite Memory.split_o in GET; eauto. des_ifs.
+      + ss. des; clarify. auto.
+      + ss. des; clarify. exploit PF; ss.
+      + eapply PROMISES; eauto.
+    - ii. erewrite Memory.lower_o in GET; eauto. des_ifs.
+      + ss. des; clarify. auto.
+      + eapply PROMISES; eauto.
+    - ii. erewrite Memory.remove_o in GET; eauto. des_ifs.
+      eapply PROMISES; eauto.
+  Qed.
+
+  Lemma pf_promises_write prom0 mem0 loc from to val released prom1 mem1 kind
+        (WRITE: Memory.write prom0 mem0 loc from to val released prom1 mem1 kind)
+        (PROMISES: pf_promises prom0)
+    :
+      pf_promises prom1.
+  Proof.
+    inv WRITE. ii. erewrite Memory.remove_o in GET; eauto. des_ifs.
+    inv PROMISE.
+    - ii. erewrite Memory.add_o in GET; eauto. des_ifs.
+      + ss. des; clarify.
+      + eapply PROMISES; eauto.
+    - ii. erewrite Memory.split_o in GET; eauto. des_ifs.
+      + ss. des; clarify.
+      + ss. des; clarify.
+        eapply Memory.split_get0 in PROMISES0. des.
+        eapply PROMISES in GET0; eauto.
+      + eapply PROMISES; eauto.
+    - ii. erewrite Memory.lower_o in GET; eauto. des_ifs.
+      + ss. des; clarify.
+      + eapply PROMISES; eauto.
+    - ii. erewrite Memory.remove_o in GET; eauto. des_ifs.
+  Qed.
+
+  Lemma pf_promises_step lang (th0 th1: Thread.t lang) pf e
+        (STEP: Thread.step pf e th0 th1)
+        (PF: pf_event e)
+        (PROMISES: pf_promises th0.(Thread.local).(Local.promises))
+    :
+      pf_promises th1.(Thread.local).(Local.promises).
+  Proof.
+    inv STEP.
+    - inv STEP0; ss. inv LOCAL.
+      eapply pf_promises_promise; eauto.
+    - inv STEP0. inv LOCAL; ss.
+      + inv LOCAL0; ss.
+      + inv LOCAL0; ss.
+        eapply pf_promises_write; eauto.
+      + inv LOCAL1. inv LOCAL2; ss.
+        eapply pf_promises_write; eauto.
+      + inv LOCAL0; ss.
+      + inv LOCAL0; ss.
+  Qed.
+
+  Lemma pf_promises_opt_step lang (th0 th1: Thread.t lang) e
+        (STEP: Thread.opt_step e th0 th1)
+        (PF: pf_event e)
+        (PROMISES: pf_promises th0.(Thread.local).(Local.promises))
+    :
+      pf_promises th1.(Thread.local).(Local.promises).
+  Proof.
+    inv STEP; auto.
+    eapply pf_promises_step; eauto.
+  Qed.
+
+  Lemma pf_promises_reserve_steps lang (th0 th1: Thread.t lang)
+        (STEPS: rtc (@Thread.reserve_step _) th0 th1)
+        (PROMISES: pf_promises th0.(Thread.local).(Local.promises))
+    :
+      pf_promises th1.(Thread.local).(Local.promises).
+  Proof.
+    ginduction STEPS; eauto. i. eapply IHSTEPS.
+    inv H. eapply pf_promises_step; eauto. ii. clarify.
+  Qed.
+
+  Lemma pf_promises_cancel_steps lang (th0 th1: Thread.t lang)
+        (STEPS: rtc (@Thread.cancel_step _) th0 th1)
+        (PROMISES: pf_promises th0.(Thread.local).(Local.promises))
+    :
+      pf_promises th1.(Thread.local).(Local.promises).
+  Proof.
+    ginduction STEPS; eauto. i. eapply IHSTEPS.
+    inv H. eapply pf_promises_step; eauto. ii. clarify.
+  Qed.
+
+  Definition pf_configuration (c: Configuration.t) :=
+    forall tid lang st lc
+           (TID: IdentMap.find tid c.(Configuration.threads) = Some (existT _ lang st, lc)),
+      pf_promises lc.(Local.promises).
+
+  Lemma configuration_init_pf syn: pf_configuration (Configuration.init syn).
+  Proof.
+    ii. ss. unfold Threads.init in *.
+    erewrite IdentMap.Facts.map_o in TID.
+    unfold option_map in *. des_ifs. dep_clarify.
+    erewrite Memory.bot_get in GET. ss.
+  Qed.
+
+  Lemma pf_configuration_step tid c1 c2 e
+        (STEP: pf_step e tid c1 c2)
+        (PF: pf_configuration c1)
+    :
+      pf_configuration c2.
+  Proof.
+    inv STEP. unfold pf_configuration in *. i. ss.
+    erewrite IdentMap.gsspec in TID0. des_ifs; eauto.
+    dep_clarify. eapply PF in TID.
+    eapply pf_promises_cancel_steps in CANCELS; eauto.
+    eapply pf_promises_opt_step in STEP0; eauto.
+    eapply pf_promises_reserve_steps in RESERVES; eauto.
+  Qed.
+
+  Lemma pf_promises_pf_step_pf_event lang (th0 th1: Thread.t lang) e
+        (STEP: Thread.step true e th0 th1)
+        (PROMISES: pf_promises th0.(Thread.local).(Local.promises))
+    :
+      pf_event e.
+  Proof.
+    ii. subst. inv STEP; inv STEP0; inv LOCAL. ss.
+    inv PROMISE; ss. des. subst.
+    eapply Memory.lower_get0 in PROMISES0. des.
+    eapply PROMISES in GET; eauto. clarify.
+  Qed.
+
+  Lemma pf_promises_pf_steps_pf_trace lang (th0 th1: Thread.t lang)
+        (STEPS: rtc (tau (Thread.step true)) th0 th1)
+        (PROMISES: pf_promises th0.(Thread.local).(Local.promises))
+    :
+      exists tr,
+        (<<STEPS: Trace.steps tr th0 th1>>) /\
+        (<<PF: List.Forall (compose pf_event snd) tr>>) /\
+        (<<SILENT: List.Forall (fun lce => ThreadEvent.get_machine_event (snd lce) = MachineEvent.silent) tr>>).
+  Proof.
+    ginduction STEPS; eauto; i.
+    { exists []. splits; eauto. }
+    i. inv H. hexploit pf_promises_pf_step_pf_event; eauto. intros PF.
+    hexploit pf_promises_step; eauto. intros PROMISES0.
+    exploit IHSTEPS; eauto. i. des. esplits; eauto.
+  Qed.
+
+  Lemma pf_promises_consistent_pf_consistent lang (th: Thread.t lang)
+        (CONSISTENT: Thread.consistent th)
+        (WF: Local.wf th.(Thread.local) th.(Thread.memory))
+        (MEM: Memory.closed th.(Thread.memory))
+        (PROMISES: pf_promises th.(Thread.local).(Local.promises))
+    :
+      pf_consistent th.
+  Proof.
+    eapply consistent_pf_consistent in CONSISTENT; eauto.
+    exploit Memory.cap_exists; eauto. i. des.
+    exploit Memory.max_concrete_timemap_exists.
+    { eapply Memory.cap_closed; eauto. } i. des.
+    exploit CONSISTENT; eauto. i. des.
+    { eapply pf_promises_pf_steps_pf_trace in STEPS; eauto. des.
+      exists tr. splits; auto. ii.
+      exploit (@Memory.cap_inj th.(Thread.memory) mem2 mem1); eauto. i. subst.
+      exploit (@Memory.max_concrete_timemap_inj mem1 tm sc1); eauto. i. subst.
+      esplits; eauto.
+    }
+    { eapply pf_promises_pf_steps_pf_trace in STEPS; eauto. des.
+      exists tr. splits; auto. ii.
+      exploit (@Memory.cap_inj th.(Thread.memory) mem2 mem1); eauto. i. subst.
+      exploit (@Memory.max_concrete_timemap_inj mem1 tm sc1); eauto. i. subst.
+      esplits; eauto.
+    }
+  Qed.
+
+  Lemma pf_event_configuration_step_pf_step c1 c2 e tid
+        (STEP: SConfiguration.step e tid c1 c2)
+        (WF: Configuration.wf c1)
+        (PF: pf_configuration c1)
+        (EVENT: pf_event e)
+    :
+      pf_step e tid c1 c2.
+  Proof.
+    inv STEP. econs; eauto. i.
+    exploit Thread.rtc_cancel_step_future; eauto; try eapply WF; eauto. ss. i. des.
+    exploit Thread.opt_step_future; eauto. ss. i. des.
+    exploit Thread.rtc_reserve_step_future; eauto; try eapply WF; eauto. ss. i. des.
+    hexploit pf_promises_cancel_steps; eauto. i. ss.
+    hexploit pf_promises_opt_step; eauto. i. ss.
+    hexploit pf_promises_reserve_steps; eauto. i. ss.
+    eapply pf_promises_consistent_pf_consistent; eauto.
+  Qed.
+
+  Lemma reservation_only_step_pf_step tid c1 c2
+        (STEP: SConfiguration.reservation_only_step tid c1 c2)
+        (WF: Configuration.wf c1)
+        (PF: pf_configuration c1)
+    :
+      pf_step ThreadEvent.silent tid c1 c2.
+  Proof.
+    eapply SConfiguration.reservation_only_step_step in STEP.
+    eapply pf_event_configuration_step_pf_step; eauto. ss.
+  Qed.
+
+  Lemma pf_step_pf_event_configuration_step c1 c2 e tid
+        (STEP: pf_step e tid c1 c2)
+        (WF: Configuration.wf c1)
+    :
+      (<<STEP: SConfiguration.step e tid c1 c2>>) /\
+      (<<EVENT: pf_event e>>)
+  .
+  Proof.
+    inv STEP. splits; auto. econs; eauto.
+    i. eapply pf_consistent_consistent; eauto.
+  Qed.
+
+  Lemma pf_step_future
+        e tid c1 c2
+        (STEP: pf_step e tid c1 c2)
+        (WF1: Configuration.wf c1)
+        (PF: pf_configuration c1):
+    (<<WF2: Configuration.wf c2>>) /\
+    (<<SC_FUTURE: TimeMap.le c1.(Configuration.sc) c2.(Configuration.sc)>>) /\
+    (<<MEM_FUTURE: Memory.future c1.(Configuration.memory) c2.(Configuration.memory)>>) /\
+    (<<PF: pf_configuration c2>>).
+  Proof.
+    exploit pf_step_pf_event_configuration_step; eauto. i. des.
+    exploit SConfiguration.step_future; eauto. i. des.
+    splits; auto. eapply pf_configuration_step; eauto.
+  Qed.
+
+  Lemma pf_machine_step_future
+        e tid c1 c2
+        (STEP: pf_machine_step e tid c1 c2)
+        (WF1: Configuration.wf c1)
+        (PF: pf_configuration c1):
+    (<<WF2: Configuration.wf c2>>) /\
+    (<<SC_FUTURE: TimeMap.le c1.(Configuration.sc) c2.(Configuration.sc)>>) /\
+    (<<MEM_FUTURE: Memory.future c1.(Configuration.memory) c2.(Configuration.memory)>>) /\
+    (<<PF: pf_configuration c2>>).
+  Proof.
+    inv STEP. eapply pf_step_future; eauto.
+  Qed.
+
+  Lemma opt_pf_machine_step_future
+        e tid c1 c2
+        (STEP: opt_pf_machine_step e tid c1 c2)
+        (WF1: Configuration.wf c1)
+        (PF: pf_configuration c1):
+    (<<WF2: Configuration.wf c2>>) /\
+    (<<SC_FUTURE: TimeMap.le c1.(Configuration.sc) c2.(Configuration.sc)>>) /\
+    (<<MEM_FUTURE: Memory.future c1.(Configuration.memory) c2.(Configuration.memory)>>) /\
+    (<<PF: pf_configuration c2>>).
+  Proof.
+    inv STEP; eauto.
+    - splits; eauto. refl.
+    - eapply pf_machine_step_future; eauto.
+  Qed.
+
+  Lemma pf_all_step_future
+        c1 c2
+        (STEP: pf_all_step c1 c2)
+        (WF1: Configuration.wf c1)
+        (PF: pf_configuration c1):
+    (<<WF2: Configuration.wf c2>>) /\
+    (<<SC_FUTURE: TimeMap.le c1.(Configuration.sc) c2.(Configuration.sc)>>) /\
+    (<<MEM_FUTURE: Memory.future c1.(Configuration.memory) c2.(Configuration.memory)>>) /\
+    (<<PF: pf_configuration c2>>).
+  Proof.
+    inv STEP. eapply pf_step_future; eauto.
+  Qed.
+
+  Lemma tau_pf_machine_step_future
+        c1 c2
+        (STEP: tau_pf_machine_step c1 c2)
+        (WF1: Configuration.wf c1)
+        (PF: pf_configuration c1):
+    (<<WF2: Configuration.wf c2>>) /\
+    (<<SC_FUTURE: TimeMap.le c1.(Configuration.sc) c2.(Configuration.sc)>>) /\
+    (<<MEM_FUTURE: Memory.future c1.(Configuration.memory) c2.(Configuration.memory)>>) /\
+    (<<PF: pf_configuration c2>>).
+  Proof.
+    inv STEP. eapply pf_machine_step_future; eauto.
+  Qed.
+
+  Lemma rtc_tau_pf_machine_step_future
+        c1 c2
+        (STEPS: rtc tau_pf_machine_step c1 c2)
+        (WF1: Configuration.wf c1)
+        (PF: pf_configuration c1):
+    (<<WF2: Configuration.wf c2>>) /\
+    (<<SC_FUTURE: TimeMap.le c1.(Configuration.sc) c2.(Configuration.sc)>>) /\
+    (<<MEM_FUTURE: Memory.future c1.(Configuration.memory) c2.(Configuration.memory)>>) /\
+    (<<PF: pf_configuration c2>>).
+  Proof.
+    ginduction STEPS; eauto.
+    - i. splits; eauto. refl.
+    - i. exploit tau_pf_machine_step_future; eauto. i. des.
+      exploit IHSTEPS; eauto. i. des. esplits; eauto. etrans; eauto.
+  Qed.
+
+  Lemma rtc_pf_all_step_future
+        c1 c2
+        (STEPS: rtc pf_all_step c1 c2)
+        (WF1: Configuration.wf c1)
+        (PF: pf_configuration c1):
+    (<<WF2: Configuration.wf c2>>) /\
+    (<<SC_FUTURE: TimeMap.le c1.(Configuration.sc) c2.(Configuration.sc)>>) /\
+    (<<MEM_FUTURE: Memory.future c1.(Configuration.memory) c2.(Configuration.memory)>>).
+  Proof.
+    ginduction STEPS; eauto.
+    - i. splits; eauto. refl.
+    - i. exploit pf_all_step_future; eauto. i. des.
+      exploit IHSTEPS; eauto. i. des. esplits; eauto. etrans; eauto.
+  Qed.
+
+  Lemma pf_steps_future
+        es tid c1 c2
+        (STEPS: pf_steps es tid c1 c2)
+        (WF1: Configuration.wf c1)
+        (PF: pf_configuration c1):
+    (<<WF2: Configuration.wf c2>>) /\
+    (<<SC_FUTURE: TimeMap.le c1.(Configuration.sc) c2.(Configuration.sc)>>) /\
+    (<<MEM_FUTURE: Memory.future c1.(Configuration.memory) c2.(Configuration.memory)>>) /\
+    (<<PF: pf_configuration c2>>).
+  Proof.
+    ginduction STEPS; eauto.
+    - i. splits; eauto. refl.
+    - i. exploit pf_step_future; eauto. i. des.
+      exploit IHSTEPS; eauto. i. des. esplits; eauto. etrans; eauto.
+  Qed.
+
+
+
+
   (* multiple thread steps per one configuration step *)
   Inductive pf_step_trace: forall (tr: Trace.t) (e:MachineEvent.t) (tid:Ident.t) (c1 c2:Configuration.t), Prop :=
   | pf_step_trace_intro
@@ -59,6 +586,46 @@ Section LOCALPF.
     :
       pf_step_trace tr (ThreadEvent.get_machine_event e) tid c1 (Configuration.mk (IdentMap.add tid (existT _ _ st3, lc3) c1.(Configuration.threads)) sc3 memory3)
   .
+
+  Lemma pf_promises_trace_steps lang (th0 th1: Thread.t lang) tr
+        (STEPS: Trace.steps tr th0 th1)
+        (PF: List.Forall (compose pf_event snd) tr)
+        (PROMISES: pf_promises th0.(Thread.local).(Local.promises))
+    :
+      pf_promises th1.(Thread.local).(Local.promises).
+  Proof.
+    ginduction STEPS; eauto. i. subst.
+    inv PF. eapply IHSTEPS; eauto.
+    eapply pf_promises_step; eauto.
+  Qed.
+
+  Lemma pf_trace_step_pf_step_trace c1 c2 tr e tid
+        (STEP: Trace.configuration_step tr e tid c1 c2)
+        (WF: Configuration.wf c1)
+        (PF: pf_configuration c1)
+        (TRACE: List.Forall (compose pf_event snd) tr)
+    :
+      pf_step_trace tr e tid c1 c2.
+  Proof.
+    inv STEP. econs; eauto. i.
+    eapply Forall_app_inv in TRACE. des. inv FORALL2.
+    exploit Trace.steps_future; eauto; try eapply WF; eauto. ss. i. des.
+    exploit Thread.step_future; eauto. ss. i. des.
+    hexploit pf_promises_trace_steps; eauto. i. ss.
+    hexploit pf_promises_step; eauto. i. ss.
+    eapply pf_promises_consistent_pf_consistent; eauto.
+  Qed.
+
+  Lemma pf_step_trace_pf_trace_step c1 c2 tr e tid
+        (STEP: pf_step_trace tr e tid c1 c2)
+        (WF: Configuration.wf c1)
+    :
+      (<<STEP: Trace.configuration_step tr e tid c1 c2>>) /\
+      (<<TRACE: List.Forall (compose pf_event snd) tr>>).
+  Proof.
+    inv STEP. splits; auto. econs; eauto. i.
+    eapply pf_consistent_consistent; eauto.
+  Qed.
 
   Inductive pf_opt_step_trace: forall (tr: Trace.t) (e:MachineEvent.t) (tid:Ident.t) (c1 c2:Configuration.t), Prop :=
   | pf_opt_step_trace_some
@@ -87,31 +654,6 @@ Section LOCALPF.
     }
   Qed.
 
-  Lemma pf_step_trace_future
-        (tr: Trace.t) e tid c1 c2
-        (STEP: pf_step_trace tr e tid c1 c2)
-        (WF1: Configuration.wf c1):
-    (<<WF2: Configuration.wf c2>>) /\
-    (<<SC_FUTURE: TimeMap.le c1.(Configuration.sc) c2.(Configuration.sc)>>) /\
-    (<<MEM_FUTURE: Memory.future c1.(Configuration.memory) c2.(Configuration.memory)>>).
-  Proof.
-    eapply pf_step_trace_step in STEP.
-    eapply Configuration.step_future; eauto.
-  Qed.
-
-  Lemma pf_opt_step_trace_future
-        (tr: Trace.t) e tid c1 c2
-        (STEP: pf_opt_step_trace tr e tid c1 c2)
-        (WF1: Configuration.wf c1):
-    (<<WF2: Configuration.wf c2>>) /\
-    (<<SC_FUTURE: TimeMap.le c1.(Configuration.sc) c2.(Configuration.sc)>>) /\
-    (<<MEM_FUTURE: Memory.future c1.(Configuration.memory) c2.(Configuration.memory)>>).
-  Proof.
-    inv STEP.
-    { eapply pf_step_trace_future; eauto. }
-    { splits; auto. refl. }
-  Qed.
-
   Inductive pf_steps_trace:
     forall (c0 c1: Configuration.t) (tr: Trace.t), Prop :=
   | pf_steps_trace_nil
@@ -126,13 +668,69 @@ Section LOCALPF.
       pf_steps_trace c0 c2 (tr ++ trs)
   .
 
+  Lemma pf_step_trace_pf_steps tr e tid c1 c3
+        (STEP: pf_step_trace tr e tid c1 c3)
+        (WF: Configuration.wf c1)
+        (PF: pf_configuration c1)
+    :
+      ((<<STEPS: pf_steps (List.filter ThreadEvent.is_normal_dec (List.map snd tr)) tid c1 c3>>) /\
+       (<<NIL: List.filter ThreadEvent.is_normal_dec (List.map snd tr) <> []>>)) \/
+      ((<<STEP: SConfiguration.reservation_only_step tid c1 c3>>) /\
+       (<<NIL: List.filter ThreadEvent.is_normal_dec (List.map snd tr) = []>>)).
+  Proof.
+    eapply pf_step_trace_pf_trace_step in STEP; eauto. des.
+    eapply SConfiguration.trace_step_machine_step in STEP0; eauto. des; eauto.
+    left. splits; auto. clear e.
+    remember (List.filter (fun e => ThreadEvent.is_normal_dec e) (List.map snd tr)).
+    assert (EVENTS: List.Forall pf_event l).
+    { subst. clear - TRACE. induction tr; ss. inv TRACE. des_ifs; eauto. }
+    clear tr Heql NIL TRACE. ginduction STEPS; eauto.
+    i. inv EVENTS.
+    eapply pf_event_configuration_step_pf_step in STEP; eauto.
+    exploit pf_step_future; eauto. i. des.
+    hexploit pf_configuration_step; eauto.
+  Qed.
+
+  Lemma pf_step_trace_future
+        (tr: Trace.t) e tid c1 c2
+        (STEP: pf_step_trace tr e tid c1 c2)
+        (WF1: Configuration.wf c1)
+        (PF: pf_configuration c1):
+    (<<WF2: Configuration.wf c2>>) /\
+    (<<SC_FUTURE: TimeMap.le c1.(Configuration.sc) c2.(Configuration.sc)>>) /\
+    (<<MEM_FUTURE: Memory.future c1.(Configuration.memory) c2.(Configuration.memory)>>) /\
+    (<<PF: pf_configuration c2>>).
+  Proof.
+    eapply pf_step_trace_pf_steps in STEP; eauto. des.
+    { eapply pf_steps_future; eauto. }
+    { eapply reservation_only_step_pf_step in STEP0; eauto.
+      eapply pf_step_future; eauto. }
+  Qed.
+
+  Lemma pf_opt_step_trace_future
+        (tr: Trace.t) e tid c1 c2
+        (STEP: pf_opt_step_trace tr e tid c1 c2)
+        (WF1: Configuration.wf c1)
+        (PF: pf_configuration c1):
+    (<<WF2: Configuration.wf c2>>) /\
+    (<<SC_FUTURE: TimeMap.le c1.(Configuration.sc) c2.(Configuration.sc)>>) /\
+    (<<MEM_FUTURE: Memory.future c1.(Configuration.memory) c2.(Configuration.memory)>>) /\
+    (<<PF: pf_configuration c2>>).
+  Proof.
+    inv STEP.
+    { eapply pf_step_trace_future; eauto. }
+    { splits; auto. refl. }
+  Qed.
+
   Lemma pf_steps_trace_future
         c1 c2 tr
         (STEPS: pf_steps_trace c1 c2 tr)
-        (WF1: Configuration.wf c1):
+        (WF1: Configuration.wf c1)
+        (PF: pf_configuration c1):
     (<<WF2: Configuration.wf c2>>) /\
     (<<SC_FUTURE: TimeMap.le c1.(Configuration.sc) c2.(Configuration.sc)>>) /\
-    (<<MEM_FUTURE: Memory.future c1.(Configuration.memory) c2.(Configuration.memory)>>).
+    (<<MEM_FUTURE: Memory.future c1.(Configuration.memory) c2.(Configuration.memory)>>) /\
+    (<<PF: pf_configuration c2>>).
   Proof.
     revert WF1. induction STEPS; i.
     - splits; ss; refl.
@@ -251,6 +849,7 @@ Section LOCALPF.
         c1 c2 tr lc e
         (STEPS: pf_steps_trace c1 c2 tr)
         (WF: Configuration.wf c1)
+        (PF: pf_configuration c1)
         (TRACE: List.In (lc, e) tr):
     exists c tr1 tid lang st1 lc1,
       (<<STEPS: pf_steps_trace c1 c tr1>>) /\
@@ -272,7 +871,7 @@ Section LOCALPF.
     splits; ss.
     apply List.in_app_or in TRACE. des; cycle 1.
     { inv TRACE; ss. inv H. esplits; eauto.
-      - apply Forall_app_inv in PF. des. ss.
+      - apply Forall_app_inv in PF0. des. ss.
       - destruct (classic (e = ThreadEvent.failure)).
         + subst. inv STEP0; inv STEP. inv LOCAL. inv LOCAL0. ss.
         + exploit CONSISTENT; eauto. i. inv x. des.
@@ -297,65 +896,85 @@ Section LOCALPF.
     }
     i. des. esplits; eauto; subst.
     - apply Forall_app_inv in SILENT. des. ss.
-    - apply Forall_app_inv in PF. des.
+    - apply Forall_app_inv in PF0. des.
       apply Forall_app_inv in FORALL1. des. ss.
   Qed.
 
-
-  Inductive pf_step (e:MachineEvent.t) (tid:Ident.t) (c1 c2:Configuration.t): Prop :=
-  | pf_step_intro
+  Inductive pf_multi_step (e:MachineEvent.t) (tid:Ident.t) (c1 c2:Configuration.t): Prop :=
+  | pf_multi_step_intro
       tr
       (STEP: pf_step_trace tr e tid c1 c2)
   .
 
-  Lemma pf_step_future
+  Lemma pf_multi_step_machine_step e tid c1 c3
+        (STEP: pf_multi_step e tid c1 c3)
+        (WF: Configuration.wf c1)
+        (PF: pf_configuration c1)
+    :
+      exists c2,
+        (<<STEPS: rtc tau_pf_machine_step c1 c2>>) /\
+        (<<STEP: opt_pf_machine_step e tid c2 c3>>).
+  Proof.
+    inv STEP. exploit pf_step_trace_pf_steps; eauto. i. des.
+    { inv STEP0.
+      rewrite List.map_app in *.
+      rewrite list_filter_app in *. ss.
+      eapply pf_steps_split in STEPS. des. exists c0. splits.
+      { eapply rtc_implies with (R1:=(pf_machine_step MachineEvent.silent tid)).
+        { clear. i. econs; eauto. }
+        eapply silent_pf_steps_tau_pf_machine_steps; eauto.
+        eapply list_filter_forall with (Q:=fun e => ThreadEvent.get_machine_event e = MachineEvent.silent); eauto.
+        eapply list_map_forall; eauto.
+      }
+      unfold proj_sumbool in *. des_ifs.
+      { inv STEPS2. inv STEPS.
+        econs 2. econs; eauto. }
+      { inv STEPS2.
+        replace (ThreadEvent.get_machine_event e0) with MachineEvent.silent; eauto.
+        apply NNPP in n.
+        unfold ThreadEvent.is_reservation_event, ThreadEvent.is_reserve, ThreadEvent.is_cancel in n.
+        des; des_ifs.
+      }
+    }
+    { eapply SConfiguration.reservation_only_step_step in STEP.
+      eapply pf_event_configuration_step_pf_step in STEP; eauto; ss.
+      exists c1. esplits; eauto.
+      replace e with (ThreadEvent.get_machine_event ThreadEvent.silent); eauto.
+      ss. inv STEP0.
+      rewrite List.map_app in NIL.
+      rewrite list_filter_app in NIL.
+      eapply List.app_eq_nil in NIL.
+      ss. unfold proj_sumbool in NIL. des. des_ifs.
+      apply NNPP in n.
+      unfold ThreadEvent.is_reservation_event, ThreadEvent.is_reserve, ThreadEvent.is_cancel in n.
+      des; des_ifs.
+    }
+  Qed.
+
+  Lemma pf_multi_step_future
         e tid c1 c2
-        (STEP: pf_step e tid c1 c2)
-        (WF1: Configuration.wf c1):
+        (STEP: pf_multi_step e tid c1 c2)
+        (WF1: Configuration.wf c1)
+        (PF: pf_configuration c1):
     (<<WF2: Configuration.wf c2>>) /\
     (<<SC_FUTURE: TimeMap.le c1.(Configuration.sc) c2.(Configuration.sc)>>) /\
-    (<<MEM_FUTURE: Memory.future c1.(Configuration.memory) c2.(Configuration.memory)>>).
+    (<<MEM_FUTURE: Memory.future c1.(Configuration.memory) c2.(Configuration.memory)>>) /\
+    (<<PF: pf_configuration c2>>).
   Proof.
     inv STEP. eapply pf_step_trace_future; eauto.
   Qed.
 
-  Lemma silent_pf_steps_trace_behaviors c0 c1 tr
+  Lemma silent_pf_multi_steps_trace_behaviors c0 c1 tr
         (STEP: silent_pf_steps_trace c0 c1 tr)
     :
-      behaviors pf_step c1 <1= behaviors pf_step c0.
+      behaviors pf_multi_step c1 <1= behaviors pf_multi_step c0.
   Proof.
     ginduction STEP; auto.
     i. eapply IHSTEP in PR. econs 4; eauto.
     econs. esplits; eauto.
   Qed.
 
-  Inductive reading_event (loc: Loc.t) (ts: Time.t):
-    forall (e: ThreadEvent.t), Prop :=
-  | reading_event_read
-      valr releasedr ordr
-    :
-      reading_event loc ts (ThreadEvent.read loc ts valr releasedr ordr)
-  | reading_event_update
-      to valr valw releasedr releasedw ordr ordw
-    :
-      reading_event loc ts (ThreadEvent.update loc ts to valr valw releasedr releasedw ordr ordw)
-  .
-
-  Inductive writing_event (loc: Loc.t) (ts: Time.t):
-    forall (e: ThreadEvent.t), Prop :=
-  | writing_event_write
-      from valw releasedw ordw
-      (ORD: Ordering.le ordw Ordering.relaxed)
-    :
-      writing_event loc ts (ThreadEvent.write loc from ts valw releasedw ordw)
-  | writing_event_update
-      from valr valw releasedr releasedw ordr ordw
-      (ORD: Ordering.le ordw Ordering.relaxed)
-    :
-      writing_event loc ts (ThreadEvent.update loc from ts valr valw releasedr releasedw ordr ordw)
-  .
-
-  Definition pf_racefree_imm (c0: Configuration.t): Prop :=
+  Definition pf_multi_racefree_imm (c0: Configuration.t): Prop :=
     forall tid0 c1 trs0 tid1 c2 trs1
            loc ts lc1 te0 te1 e0 e1
            (LOC: L loc)
@@ -368,32 +987,142 @@ Section LOCALPF.
            (TRACE1: List.In (lc1, te1) trs1),
       False.
 
-  Definition pf_racefree (c0: Configuration.t): Prop :=
+  Definition pf_multi_racefree (c0: Configuration.t): Prop :=
     forall c1 trs
            (CSTEPS: pf_steps_trace c0 c1 trs),
-      pf_racefree_imm c1.
+      pf_multi_racefree_imm c1.
 
-  Lemma step_pf_racefree c0 c1 tr e tid
-        (RACEFREE: pf_racefree c0)
+  Lemma multi_step_pf_multi_racefree c0 c1 tr e tid
+        (RACEFREE: pf_multi_racefree c0)
         (STEP: pf_step_trace tr e tid c0 c1)
     :
-      pf_racefree c1.
+      pf_multi_racefree c1.
   Proof.
-    unfold pf_racefree in *. i.
+    unfold pf_multi_racefree in *. i.
     eapply RACEFREE. econs 2; eauto.
   Qed.
 
-  Lemma steps_pf_racefree c0 c1 trs
-        (RACEFREE: pf_racefree c0)
+  Lemma multi_steps_pf_multi_racefree c0 c1 trs
+        (RACEFREE: pf_multi_racefree c0)
         (STEPS: pf_steps_trace c0 c1 trs)
     :
-      pf_racefree c1.
+      pf_multi_racefree c1.
   Proof.
     induction STEPS; auto. eapply IHSTEPS.
-    eapply step_pf_racefree; eauto.
+    eapply multi_step_pf_multi_racefree; eauto.
   Qed.
 
+  Lemma reserving_trace_filter tr
+        (TRACE: reserving_trace tr)
+    :
+      List.filter ThreadEvent.is_normal_dec (List.map snd tr) = [].
+  Proof.
+    induction TRACE; eauto. ss. rewrite IHTRACE; eauto.
+    unfold ThreadEvent.is_normal, proj_sumbool in *. des_ifs.
+  Qed.
 
+  Lemma final_event_trace_filter tr e
+        (FINAL: final_event_trace e tr)
+        (NORMAL: ThreadEvent.is_normal e)
+    :
+      exists tr_hd,
+        (<<FILTER: List.filter ThreadEvent.is_normal_dec (List.map snd tr) = tr_hd ++ [e]>>).
+  Proof.
+    induction FINAL; eauto; i.
+    { exists []. ss. rewrite reserving_trace_filter; eauto.
+      unfold proj_sumbool. des_ifs. }
+    { des. ss. rewrite FILTER. des_ifs; eauto.
+      eexists. erewrite List.app_comm_cons. eauto.
+    }
+  Qed.
+
+  Lemma pf_racefree_multi_racefree_imm c
+        (RACEFREE: pf_racefree c)
+        (WF: Configuration.wf c)
+        (PF: pf_configuration c)
+    :
+      pf_multi_racefree_imm c.
+  Proof.
+    ii. exploit pf_step_trace_future; try apply CSTEP0; eauto.  i. des.
+    exploit final_event_trace_filter; eauto.
+    { unfold ThreadEvent.is_normal, ThreadEvent.is_reservation_event.
+      inv WRITE; ss; ii; des; ss. } i. des.
+    eapply pf_step_trace_pf_steps in CSTEP0; eauto.
+    rewrite FILTER in *. des; cycle 1.
+    { eapply List.app_eq_nil in NIL. des; ss. }
+    eapply pf_steps_split in STEPS. des. inv STEPS1. inv STEPS.
+    eapply List.in_split in TRACE1. des; subst.
+    dup CSTEP1. eapply pf_step_trace_pf_steps in CSTEP1; eauto.
+    rewrite List.map_app in *.
+    rewrite list_filter_app in *. ss. unfold proj_sumbool in *.
+    des_ifs; cycle 1.
+    { clear - READ n. apply NNPP in n.
+      unfold ThreadEvent.is_normal, ThreadEvent.is_reservation_event in *.
+      inv READ; ss; ii; des; ss. }
+    des; cycle 1.
+    { eapply List.app_eq_nil in NIL0. des; ss. }
+    eapply pf_steps_split in STEPS. des. inv STEPS2.
+    eapply RACEFREE; try eassumption.
+    { eapply pf_steps_rtc_pf_all_step; eauto. }
+    { eapply silent_pf_steps_tau_pf_machine_steps; eauto.
+      clear - CSTEP0. inv CSTEP0.
+      destruct (list_match_rev l2); des; subst.
+      { eapply List.app_inj_tail in TR. des; clarify.
+        eapply List.Forall_forall. ii.
+        eapply List.filter_In in H. des.
+        eapply List.in_map_iff in H. des; subst.
+        eapply List.Forall_forall in SILENT; eauto. }
+      { rewrite List.app_comm_cons in TR.
+        rewrite List.app_assoc in TR.
+        eapply List.app_inj_tail in TR. des; clarify.
+        eapply Forall_app_inv in SILENT. des.
+        eapply List.Forall_forall. ii.
+        eapply List.filter_In in H. des.
+        eapply List.in_map_iff in H. des; subst.
+        eapply List.Forall_forall in FORALL1; eauto. }
+    }
+  Qed.
+
+  Lemma pf_racefree_multi_racefree c
+        (RACEFREE: pf_racefree c)
+        (WF: Configuration.wf c)
+        (PF: pf_configuration c)
+    :
+      pf_multi_racefree c.
+  Proof.
+    unfold pf_multi_racefree. i.
+    ginduction CSTEPS; eauto.
+    { i. eapply pf_racefree_multi_racefree_imm; eauto. }
+    { i. exploit pf_step_trace_future; eauto.
+      i. des. eapply IHCSTEPS; eauto.
+      eapply pf_step_trace_pf_steps in STEP; eauto. des.
+      { eapply steps_pf_racefree; eauto. }
+      { eapply reservation_only_step_pf_step in STEP0; eauto.
+        eapply step_pf_racefree; eauto. }
+    }
+  Qed.
+
+  Lemma pf_multi_step_behavior c
+        (WF: Configuration.wf c)
+        (PF: pf_configuration c)
+    :
+      behaviors pf_multi_step c <1= behaviors pf_machine_step c.
+  Proof.
+    i. induction PR.
+    - econs 1; eauto.
+    - exploit pf_multi_step_future; eauto. i. des.
+      eapply pf_multi_step_machine_step in STEP; eauto. des.
+      eapply rtc_tau_step_behavior; eauto.
+      inv STEP0; eauto. econs 2; eauto.
+    - exploit pf_multi_step_future; eauto. i. des.
+      eapply pf_multi_step_machine_step in STEP; eauto. des.
+      eapply rtc_tau_step_behavior; eauto.
+      inv STEP0; eauto. econs 3; eauto.
+    - exploit pf_multi_step_future; eauto. i. des.
+      eapply pf_multi_step_machine_step in STEP; eauto. des.
+      eapply rtc_tau_step_behavior; eauto.
+      inv STEP0; eauto. econs 4; eauto.
+  Qed.
 
   Inductive racy_read (loc: Loc.t) (ts: Time.t):
     forall (lc: Local.t) (e: ThreadEvent.t), Prop :=
